lib/seq: some preliminary results for Count, Subseq, Undup

lib/math/Gcd.dfy
@@ -1,21 +1,19 @@
 include "Abs.dfy"
 
-function {:opaque} Gcd(a: int, b: int): int
+function method {:opaque} Gcd(a: int, b: int): int
   decreases Abs(b)
 {
-  if b == 0 then Abs(a) else Gcd(b, a % b)
+  if b != 0 then Gcd(b, a % b) else if a == 0 then 1 else Abs(a)
 }
 
-lemma GcdPos(a: int, b: int)
-  requires a != 0 || b != 0
-  ensures 0 < Gcd(a, b)
-  decreases Abs(b)
+lemma Gcd00()
+  ensures Gcd(0, 0) == 1
 {
   reveal Gcd();
 }
 
-lemma Gcd0(a: int, b: int)
-  ensures Gcd(a, b) == 0 <==> a == 0 && b == 0
+lemma GcdPos(a: int, b: int)
+  ensures 0 < Gcd(a, b)
   decreases Abs(b)
 {
   reveal Gcd();
@@ -30,8 +28,9 @@ lemma AddMod(a: int, b: int, c: int)
   ensures (a + b) % c == (a % c + b % c) % c
 
 lemma GcdIsDivisor(a: int, b: int)
-  requires a != 0 || b != 0
-  ensures 0 < Gcd(a, b) && a % Gcd(a, b) == 0 && b % Gcd(a, b) == 0
+  ensures 0 < Gcd(a, b)
+  ensures a % Gcd(a, b) == 0 && b % Gcd(a, b) == 0
+  // ensures forall c :: c != 0 && a % c == 0 && b % c == 0 ==> Gcd(a, b) % c == 0
   decreases Abs(b)
 {
   if b == 0 {
@@ -55,3 +54,22 @@ lemma GcdIsDivisor(a: int, b: int)
     }
   }
 }
+
+lemma GcdSym(a: int, b: int)
+  ensures Gcd(a, b) == Gcd(b, a)
+  decreases Abs(b)
+// {
+//   if b == 0 || a == 0 {
+//     reveal Gcd();
+//   } else {
+//     assert Gcd(a, b) == Gcd(b, a % b) by {
+//       reveal Gcd();
+//     }
+//     assert Gcd(b, a) == Gcd(a, b % a) by {
+//       reveal Gcd();
+//     }
+//     GcdSym(b, a % b);
+//     GcdSym(a, b % a);
+//     assert Gcd(b, a % b) == Gcd(a % b, b);
+//   }
+// }
