leetcode/[wip]0027-remove-element.dfy
@@ -1,11 +1,11 @@
 include "../lib/Seq.dfy"
-// include "../lib/WorkCount.dfy"
+include "../lib/seq/Count.dfy"
 
 import opened Seq
 
-function Count<T>(xs: seq<T>, v: T): int {
-  Foldl'((r, x)=> r + (if x == v then 1 else 0), 0, xs)
-}
+// function Count<T>(xs: seq<T>, v: T): int {
+//   Foldl'((r, x)=> r + (if x == v then 1 else 0), 0, xs)
+// }
 
 // TODO: ensure that multiplicities of elements are preserved
 method RemoveElement(nums: array<int>, val: int) returns (length: nat)
