lib/seq/Undup.dfy
@@ -1,0 +1,40 @@
+include "../Seq.dfy"
+
+import opened Seq
+
+function {:opaque} Undup<T>(xs: seq<T>): seq<T> {
+  if |xs| == 0 then xs 
+  else if Last(xs) in RemoveLast(xs) then Undup(RemoveLast(xs))
+  else Undup(RemoveLast(xs)) + [Last(xs)]
+}
+
+lemma MemUndup<T>(xs: seq<T>)
+  ensures forall x :: x in Undup(xs) <==> x in xs
+{
+  reveal Undup();
+}
+
+lemma DistinctUndup<T>(xs: seq<T>)
+  ensures Distinct(Undup(xs))
+{
+  reveal Undup();
+  if |xs| != 0 && Last(xs) !in RemoveLast(xs) {
+    MemUndup(RemoveLast(xs));
+  }
+}
+
+// lemma SubseqUndup<T>(xs: seq<T>)
+//   ensures Subseq(Undup(xs), xs)
+// {
+//   reveal Subseq();
+//   reveal Undup();
+//   if |xs| == 0 {
+//   } else if Last(xs) in RemoveLast(xs) {
+//     SubseqRemoveLast(xs);
+//     SubseqTrans(Undup(xs), RemoveLast(xs), xs);
+//   } else {
+
+//     // SubseqRemoveLast(xs);
+//     // assume false;
+//   }
+// }
